x64 refine: arch-split up to InvariantUpdates_H
Updates the rest of X64 Refine to conform to the generic arch-split
invariant interface. When things broke and when possible, we took the
proof or chunks of proof from AARCH64.

Otherwise:
- projectKOs is not in the simpset
- ioport_control/valid_arch_mdb_ctes hasn't been renamed in all cases, only
  made to work for now
- the power-of-two vs mask situation is still a mess, requiring changing
  proofs to go one way or the other
- unfolding tcb_cte_cases_def would benefit from tcb_cte_cases_neqs
  being in the simpset so that people avoid unfolding cteSizeBits when
  not necessary, but that can be done via a separate pass later

Signed-off-by: Rafal Kolanski <rafal.kolanski@proofcraft.systems>

proof/refine/X64/ArchInvsDefs_H.thy
@@ -37,200 +37,274 @@ end
 
 context Arch begin arch_global_naming
 
-declare lookupPTSlotFromLevel.simps[simp del]
-declare lookupPTFromLevel.simps[simp del]
-
-(* this architecture does not use kernel_mappings / pspace_in_kernel_mappings *)
-definition kernel_mappings :: "machine_word set" where
-  "kernel_mappings \<equiv> UNIV"
-
-definition pspace_in_kernel_mappings' :: "kernel_state \<Rightarrow> bool" where
- "pspace_in_kernel_mappings' \<equiv> \<top>"
-
-(* FIXME arch-split: if pspace_in_kernel_mappings becomes part of generic interface,
-   check whether having this simp is still beneficial *)
-lemmas [simp] = pspace_in_kernel_mappings'_def kernel_mappings_def
-
-abbreviation vcpu_at' :: "obj_ref \<Rightarrow> kernel_state \<Rightarrow> bool" where
-  "vcpu_at' \<equiv> typ_at' (ArchT VCPUT)"
-
-abbreviation pte_at' :: "obj_ref \<Rightarrow> kernel_state \<Rightarrow> bool" where
+abbreviation
+  "pde_at' \<equiv> typ_at' (ArchT PDET)"
+abbreviation
   "pte_at' \<equiv> typ_at' (ArchT PTET)"
+abbreviation
+  "pdpte_at' \<equiv> typ_at' (ArchT PDPTET)"
+abbreviation
+  "pml4e_at' \<equiv> typ_at' (ArchT PML4ET)"
 
 (* hyp_refs *)
 
-definition tcb_vcpu_refs' :: "machine_word option \<Rightarrow> (obj_ref \<times> reftype) set" where
-  "tcb_vcpu_refs' t \<equiv> set_option t \<times> {TCBHypRef}"
-
 definition tcb_hyp_refs' :: "arch_tcb \<Rightarrow> (obj_ref \<times> reftype) set" where
-  "tcb_hyp_refs' t \<equiv> tcb_vcpu_refs' (AARCH64_H.atcbVCPUPtr t)"
-
-definition vcpu_tcb_refs' :: "obj_ref option \<Rightarrow> (obj_ref \<times> reftype) set" where
-  "vcpu_tcb_refs' t \<equiv> set_option t \<times> {HypTCBRef}"
+  "tcb_hyp_refs' t \<equiv> {}" \<comment> \<open>no VCPUs on this architecture\<close>
 
 definition refs_of_a' :: "arch_kernel_object \<Rightarrow> (obj_ref \<times> reftype) set" where
-  "refs_of_a' x \<equiv> case x of
-     AARCH64_H.KOASIDPool asidpool \<Rightarrow> {}
-   | AARCH64_H.KOPTE pte \<Rightarrow> {}
-   | AARCH64_H.KOVCPU vcpu \<Rightarrow> vcpu_tcb_refs' (AARCH64_H.vcpuTCBPtr vcpu)"
+  "refs_of_a' x \<equiv> {}"
 
 definition arch_live' :: "arch_kernel_object \<Rightarrow> bool" where
-  "arch_live' ao \<equiv> case ao of
-     AARCH64_H.KOVCPU vcpu \<Rightarrow> bound (AARCH64_H.vcpuTCBPtr vcpu)
-   | _ \<Rightarrow>  False"
+  "arch_live' ao \<equiv> False"
 
 definition hyp_live' :: "kernel_object \<Rightarrow> bool" where
-  "hyp_live' ko \<equiv> case ko of
-     (KOTCB tcb) \<Rightarrow> bound (AARCH64_H.atcbVCPUPtr (tcbArch tcb))
-   | (KOArch ako) \<Rightarrow> arch_live' ako
-   |  _ \<Rightarrow> False"
+  "hyp_live' ko \<equiv> False"
 
-primrec azobj_refs' :: "arch_capability \<Rightarrow> obj_ref set" where
-  "azobj_refs' (ASIDPoolCap _ _) = {}"
-| "azobj_refs' ASIDControlCap = {}"
-| "azobj_refs' (FrameCap _ _ _ _ _) = {}"
-| "azobj_refs' (PageTableCap _ _ _) = {}"
-| "azobj_refs' (VCPUCap v) = {v}"
+definition azobj_refs' :: "arch_capability \<Rightarrow> obj_ref set" where
+  "azobj_refs' _ = {}"
 
-lemma azobj_refs'_only_vcpu:
-  "(x \<in> azobj_refs' acap) = (acap = VCPUCap x)"
-  by (cases acap) auto
+(* FIXME arch-split: might need to add more here, non-arch-split X64 proofs don't know these yet *)
+lemmas [simp] = refs_of_a'_def azobj_refs'_def
 
 
 section "Valid caps and objects (design spec)"
 
 primrec acapBits :: "arch_capability \<Rightarrow> nat" where
-  "acapBits (ASIDPoolCap _ _)       = asidLowBits + word_size_bits"
-| "acapBits ASIDControlCap          = asidHighBits + word_size_bits"
-| "acapBits (FrameCap _ _ sz _ _)   = pageBitsForSize sz"
-| "acapBits (PageTableCap _ pt_t _) = table_size pt_t"
-| "acapBits (VCPUCap v)             = vcpuBits"
+  "acapBits (ASIDPoolCap x y) = asidLowBits + word_size_bits"
+| "acapBits ASIDControlCap = asidHighBits + word_size_bits"
+| "acapBits (PageCap x y typ sz d z) = pageBitsForSize sz"
+| "acapBits (PageTableCap x y) = table_size"
+| "acapBits (PageDirectoryCap x y) = table_size"
+| "acapBits (PDPointerTableCap x y) = table_size"
+| "acapBits (PML4Cap x y) = table_size"
+| "acapBits (IOPortCap f l) = 0"
+| "acapBits IOPortControlCap = 0"
 
-definition page_table_at' :: "pt_type \<Rightarrow> obj_ref \<Rightarrow> kernel_state \<Rightarrow> bool" where
- "page_table_at' pt_t p \<equiv> \<lambda>s.
-    is_aligned p (ptBits pt_t) \<and>
-    (\<forall>i \<le> mask (ptTranslationBits pt_t). pte_at' (p + (i << pte_bits)) s)"
+definition
+  page_table_at' :: "machine_word \<Rightarrow> kernel_state \<Rightarrow> bool"
+where
+ "page_table_at' x \<equiv> \<lambda>s. is_aligned x ptBits
+                      \<and> (\<forall>y < 2 ^ ptTranslationBits. typ_at' (ArchT PTET) (x + (y << word_size_bits)) s)"
 
-lemmas vspace_table_at'_defs = page_table_at'_def
+definition
+  page_directory_at' :: "machine_word \<Rightarrow> kernel_state \<Rightarrow> bool"
+where
+ "page_directory_at' x \<equiv> \<lambda>s. is_aligned x pdBits
+                      \<and> (\<forall>y < 2 ^ ptTranslationBits. typ_at' (ArchT PDET) (x + (y << word_size_bits)) s)"
 
-abbreviation asid_pool_at' :: "obj_ref \<Rightarrow> kernel_state \<Rightarrow> bool" where
+definition
+  pd_pointer_table_at' :: "machine_word \<Rightarrow> kernel_state \<Rightarrow> bool"
+where
+ "pd_pointer_table_at' x \<equiv> \<lambda>s. is_aligned x pdptBits
+                      \<and> (\<forall>y < 2 ^ ptTranslationBits. typ_at' (ArchT PDPTET) (x + (y << word_size_bits)) s)"
+
+definition
+  page_map_l4_at' :: "machine_word \<Rightarrow> kernel_state \<Rightarrow> bool"
+where
+ "page_map_l4_at' x \<equiv> \<lambda>s. is_aligned x pml4Bits
+                      \<and> (\<forall>y < 2 ^ ptTranslationBits. typ_at' (ArchT PML4ET) (x + (y << word_size_bits)) s)"
+
+lemmas vspace_table_at'_defs
+  = page_table_at'_def page_directory_at'_def pd_pointer_table_at'_def page_map_l4_at'_def
+
+abbreviation
   "asid_pool_at' \<equiv> typ_at' (ArchT ASIDPoolT)"
 
-definition asid_wf :: "asid \<Rightarrow> bool" where
-  "asid_wf asid \<equiv> asid \<le> mask asid_bits"
-
-definition wellformed_mapdata' :: "asid \<times> vspace_ref \<Rightarrow> bool" where
-  "wellformed_mapdata' \<equiv> \<lambda>(asid, vref). 0 < asid \<and> asid_wf asid \<and> vref \<in> user_region"
-
-definition wellformed_acap' :: "arch_capability \<Rightarrow> bool" where
-  "wellformed_acap' ac \<equiv>
-   case ac of
-     ASIDPoolCap r asid \<Rightarrow> is_aligned asid asid_low_bits \<and> asid_wf asid
-   | FrameCap r rghts sz dev  mapdata \<Rightarrow>
-       case_option True wellformed_mapdata' mapdata \<and>
-       case_option True (swp vmsz_aligned sz \<circ> snd) mapdata
-   | PageTableCap pt_t r (Some mapdata) \<Rightarrow> wellformed_mapdata' mapdata
-   | _ \<Rightarrow> True"
-
-lemmas wellformed_acap'_simps[simp] = wellformed_acap'_def[split_simps arch_capability.split]
-
-definition frame_at' :: "obj_ref \<Rightarrow> vmpage_size \<Rightarrow> bool \<Rightarrow> kernel_state \<Rightarrow> bool" where
-  "frame_at' r sz dev s \<equiv>
-     \<forall>p < 2 ^ (pageBitsForSize sz - pageBits).
-       typ_at' (if dev then UserDataDeviceT else UserDataT) (r + (p << pageBits)) s"
-
-definition valid_arch_cap_ref' :: "arch_capability \<Rightarrow> kernel_state \<Rightarrow> bool" where
-  "valid_arch_cap_ref' ac s \<equiv> case ac of
-     ASIDPoolCap r as \<Rightarrow> typ_at' (ArchT ASIDPoolT) r s
-   | ASIDControlCap \<Rightarrow> True
-   | FrameCap r rghts sz dev mapdata \<Rightarrow> frame_at' r sz dev s
-   | PageTableCap r pt_t mapdata \<Rightarrow> page_table_at' pt_t r s
-   | VCPUCap r \<Rightarrow> vcpu_at' r s"
-
-lemmas valid_arch_cap_ref'_simps[simp] =
-  valid_arch_cap_ref'_def[split_simps arch_capability.split]
+(* FIXME arch-split: no wellformed_acap' on X64 *)
 
 definition valid_arch_cap' :: "arch_capability \<Rightarrow> kernel_state \<Rightarrow> bool" where
-  "valid_arch_cap' cap \<equiv> \<lambda>s. wellformed_acap' cap \<and> valid_arch_cap_ref' cap s"
+  "valid_arch_cap' acap s \<equiv> case acap
+   of ASIDPoolCap pool asid \<Rightarrow>
+        typ_at' (ArchT ASIDPoolT) pool s \<and> is_aligned asid asid_low_bits \<and> asid_wf asid
+    | ASIDControlCap \<Rightarrow> True
+    | PageCap ref rghts t sz d mapdata \<Rightarrow> ref \<noteq> 0 \<and>
+        (\<forall>p < 2 ^ (pageBitsForSize sz - pageBits). typ_at' (if d then UserDataDeviceT else UserDataT)
+        (ref + p * 2 ^ pageBits) s) \<and>
+        (case mapdata of None \<Rightarrow> (t=VMNoMap) | Some (asid, ref) \<Rightarrow>
+                (t = VMVSpaceMap) \<and> 0 < asid \<and> asid_wf asid \<and> vmsz_aligned ref sz \<and> ref < pptrBase)
+    | PageTableCap ref mapdata \<Rightarrow>
+        page_table_at' ref s \<and>
+        (case mapdata of None \<Rightarrow> True | Some (asid, ref) \<Rightarrow>
+                0 < asid \<and> asid_wf asid \<and> ref < pptrBase)
+    | PageDirectoryCap ref mapdata \<Rightarrow>
+        page_directory_at' ref s \<and>
+        (case mapdata of None \<Rightarrow> True | Some (asid, ref) \<Rightarrow> 0 < asid \<and> asid_wf asid \<and> ref < pptrBase)
+    | PDPointerTableCap ref mapdata \<Rightarrow>
+        pd_pointer_table_at' ref s \<and>
+        (case mapdata of None \<Rightarrow> True | Some (asid, ref) \<Rightarrow> 0 < asid \<and> asid_wf asid \<and> ref < pptrBase)
+    | PML4Cap ref mapdata \<Rightarrow>
+        page_map_l4_at' ref s \<and>
+        case_option True (\<lambda>asid. 0 < asid \<and> asid_wf asid) mapdata
+    | IOPortCap first l \<Rightarrow> first \<le> l
+    | IOPortControlCap \<Rightarrow> True"
 
 lemmas valid_arch_cap'_simps[simp] =
-  valid_arch_cap'_def[unfolded wellformed_acap'_def valid_arch_cap_ref'_def,
-                      split_simps arch_capability.split, simplified]
-
-definition is_device_frame_cap' :: "capability \<Rightarrow> bool" where
-  "is_device_frame_cap' cap \<equiv> case cap of ArchObjectCap (FrameCap _ _ _ dev _) \<Rightarrow> dev | _ \<Rightarrow> False"
+  valid_arch_cap'_def[split_simps arch_capability.split, simplified]
 
 definition valid_arch_tcb' :: "Structures_H.arch_tcb \<Rightarrow> kernel_state \<Rightarrow> bool" where
-  "valid_arch_tcb' \<equiv> \<lambda>t s. \<forall>v. atcbVCPUPtr t = Some v \<longrightarrow> vcpu_at' v s "
+  "valid_arch_tcb' \<equiv> \<lambda>t. \<top>"
 
-definition valid_vcpu' :: "vcpu \<Rightarrow> bool" where
-  "valid_vcpu' v \<equiv> case vcpuTCBPtr v of None \<Rightarrow> True | Some vt \<Rightarrow> is_aligned vt tcbBlockSizeBits"
+definition valid_mapping' :: "machine_word \<Rightarrow> vmpage_size \<Rightarrow> kernel_state \<Rightarrow> bool" where
+ "valid_mapping' x sz s \<equiv> is_aligned x (pageBitsForSize sz)
+                            \<and> ptrFromPAddr x \<noteq> 0"
 
-(* This is a slight abuse of "canonical_address". What we really need to know for ADT_C in CRefine
-   is that the top pageBits bits of TablePTEs have a known value, because we shift left by pageBits.
-   What we actually know is that this is a physical address, so it is bound by the physical address
-   space size, which depending on config can be 40, 44, or 48. 48 happens to also be the bound for
-   the virtual address space, which canonical_address is for. This is good enough for our purposes. *)
-definition ppn_bounded :: "pte \<Rightarrow> bool" where
-  "ppn_bounded pte \<equiv> case pte of PageTablePTE ppn \<Rightarrow> canonical_address ppn | _ \<Rightarrow> True"
+primrec valid_pte' :: "X64_H.pte \<Rightarrow> kernel_state \<Rightarrow> bool" where
+  "valid_pte' (InvalidPTE) = \<top>"
+| "valid_pte' (SmallPagePTE ptr _ _ _ _ _ _ _ _) = (valid_mapping' ptr X64SmallPage)"
 
-definition valid_arch_obj' :: "arch_kernel_object \<Rightarrow> kernel_state \<Rightarrow> bool" where
-  "valid_arch_obj' ako _ \<equiv> case ako of
-     KOPTE pte \<Rightarrow> ppn_bounded pte
-   | KOVCPU vcpu \<Rightarrow> valid_vcpu' vcpu
-   | _ \<Rightarrow> True"
+primrec valid_pde' :: "X64_H.pde \<Rightarrow> kernel_state \<Rightarrow> bool" where
+ "valid_pde' (InvalidPDE) = \<top>"
+| "valid_pde' (LargePagePDE ptr _ _ _ _ _ _ _ _) = (valid_mapping' ptr X64LargePage)"
+| "valid_pde' (PageTablePDE ptr _ _ _ _ _) = (\<lambda>_. is_aligned ptr ptBits)"
 
-primrec
-  acapClass :: "arch_capability \<Rightarrow> capclass"
-where
-  "acapClass (ASIDPoolCap _ _)    = PhysicalClass"
-| "acapClass ASIDControlCap       = ASIDMasterClass"
-| "acapClass (FrameCap _ _ _ _ _) = PhysicalClass"
-| "acapClass (PageTableCap _ _ _) = PhysicalClass"
-| "acapClass (VCPUCap _) = PhysicalClass"
+primrec valid_pdpte' :: "X64_H.pdpte \<Rightarrow> kernel_state \<Rightarrow> bool" where
+ "valid_pdpte' (InvalidPDPTE) = \<top>"
+| "valid_pdpte' (HugePagePDPTE ptr _ _ _ _ _ _ _ _) = (valid_mapping' ptr X64HugePage)"
+| "valid_pdpte' (PageDirectoryPDPTE ptr _ _ _ _ _) = (\<lambda>_. is_aligned ptr pdBits)"
+
+primrec valid_pml4e' :: "X64_H.pml4e \<Rightarrow> kernel_state \<Rightarrow> bool" where
+ "valid_pml4e' (InvalidPML4E) = \<top>"
+| "valid_pml4e' (PDPointerTablePML4E ptr _ _ _ _ _) = (\<lambda>_. is_aligned ptr pdptBits)"
+
+primrec valid_asid_pool' :: "asidpool \<Rightarrow> kernel_state \<Rightarrow> bool" where
+ "valid_asid_pool' (ASIDPool pool)
+     = (\<lambda>s. dom pool \<subseteq> {0 .. 2^asid_low_bits - 1}
+           \<and> 0 \<notin> ran pool \<and> (\<forall>x \<in> ran pool. is_aligned x pml4Bits))"
+
+primrec valid_arch_obj' :: "arch_kernel_object \<Rightarrow> kernel_state \<Rightarrow> bool" where
+  "valid_arch_obj' (KOASIDPool pool) = valid_asid_pool' pool"
+| "valid_arch_obj' (KOPDE pde) = valid_pde' pde"
+| "valid_arch_obj' (KOPTE pte) = valid_pte' pte"
+| "valid_arch_obj' (KOPDPTE pdpte) = valid_pdpte' pdpte"
+| "valid_arch_obj' (KOPML4E pml4e) = valid_pml4e' pml4e"
+
+definition pspace_in_kernel_mappings' :: "kernel_state \<Rightarrow> bool" where
+ "pspace_in_kernel_mappings' s \<equiv> \<forall>p \<in> dom (ksPSpace s). p \<in> kernel_mappings"
+
+primrec acapClass :: "arch_capability \<Rightarrow> capclass" where
+  "acapClass (ASIDPoolCap x y)      = PhysicalClass"
+| "acapClass ASIDControlCap         = ASIDMasterClass"
+| "acapClass (PageCap x y t sz d z) = PhysicalClass"
+| "acapClass (PageTableCap x y)     = PhysicalClass"
+| "acapClass (PageDirectoryCap x y) = PhysicalClass"
+| "acapClass (PDPointerTableCap x y) = PhysicalClass"
+| "acapClass (PML4Cap x y) = PhysicalClass"
+| "acapClass (IOPortCap x y) = IOPortClass"
+| "acapClass IOPortControlCap = IOPortClass"
+
+(* IOPortControl caps are unique and always revocable *)
+definition
+  "ioport_control m \<equiv>
+  \<forall>p n. m p = Some (CTE (ArchObjectCap IOPortControlCap) n) \<longrightarrow>
+        mdbRevocable n \<and>
+        (\<forall>p' n'. m p' = Some (CTE (ArchObjectCap IOPortControlCap) n') \<longrightarrow> p' = p)"
 
 definition
   isArchFrameCap :: "capability \<Rightarrow> bool"
 where
- "isArchFrameCap cap \<equiv> case cap of ArchObjectCap (FrameCap _ _ _ _ _) \<Rightarrow> True | _ \<Rightarrow> False"
+ "isArchFrameCap cap \<equiv> case cap of ArchObjectCap (PageCap ref rghts typ sz d data) \<Rightarrow> True | _ \<Rightarrow> False"
+
+(* FIXME arch-split: compatibility shim, can be removed by arch-wide rename *)
+abbreviation (input)
+  "isArchPageCap \<equiv> isArchFrameCap"
+
+lemmas isArchPageCap_def = isArchFrameCap_def
+
+definition
+  isArchIOPortCap :: "capability \<Rightarrow> bool"
+where
+  "isArchIOPortCap cap \<equiv> case cap of ArchObjectCap (IOPortCap f l) \<Rightarrow> True | _ \<Rightarrow> False"
 
 definition valid_arch_mdb_ctes :: "cte_heap \<Rightarrow> bool" where
-  "valid_arch_mdb_ctes \<equiv> \<top>"
+  "valid_arch_mdb_ctes \<equiv> ioport_control"
 
-(* Addresses of all PTEs in a VSRoot table at p *)
+lemmas [simp] = valid_arch_mdb_ctes_def
+
 definition table_refs' :: "machine_word \<Rightarrow> machine_word set" where
-  "table_refs' p \<equiv> (\<lambda>i. p + (i << pte_bits)) ` mask_range 0 (ptTranslationBits VSRootPT_T)"
+  "table_refs' x \<equiv> (\<lambda>y. x + (y << word_size_bits)) ` {y. y < 2^ptTranslationBits}"
 
 definition global_refs' :: "kernel_state \<Rightarrow> obj_ref set" where
   "global_refs' \<equiv> \<lambda>s.
-   {ksIdleThread s} \<union>
-   table_refs' (armKSGlobalUserVSpace (ksArchState s)) \<union>
-   range (\<lambda>irq :: irq. irq_node' s + (ucast irq << cteSizeBits))"
+  {ksIdleThread s} \<union>
+   table_refs' (x64KSSKIMPML4 (ksArchState s)) \<union>
+   (\<Union>pt \<in> set (x64KSSKIMPDs (ksArchState s)). table_refs' pt) \<union>
+   (\<Union>pt \<in> set (x64KSSKIMPTs (ksArchState s)). table_refs' pt) \<union>
+   (\<Union>pt \<in> set (x64KSSKIMPDPTs (ksArchState s)). table_refs' pt) \<union>
+   range (\<lambda>irq :: irq. irq_node' s + 32 * ucast irq)"
 
-definition valid_asid_table' :: "(asid \<rightharpoonup> machine_word) \<Rightarrow> bool" where
-  "valid_asid_table' table \<equiv> dom table \<subseteq> mask_range 0 asid_high_bits \<and> 0 \<notin> ran table"
+definition valid_asid_table' :: "(asid \<rightharpoonup> machine_word) \<Rightarrow> kernel_state \<Rightarrow> bool" where
+  "valid_asid_table' table \<equiv> \<lambda>s. dom table \<subseteq> {0 .. 2^asid_high_bits - 1}
+                                 \<and> 0 \<notin> ran table"
 
-definition "is_vcpu' \<equiv> \<lambda>ko. \<exists>vcpu. ko = (KOArch (KOVCPU vcpu))"
+primrec valid_cr3' :: "cr3 \<Rightarrow> bool" where
+  "valid_cr3' (CR3 addr pcid) = (is_aligned addr asid_bits
+                                   \<and> addr \<le> mask (pml4ShiftBits + asid_bits)
+                                   \<and> asid_wf pcid)"
 
-definition max_armKSGICVCPUNumListRegs :: nat where
-  "max_armKSGICVCPUNumListRegs \<equiv> 63"
+definition
+  valid_global_pts' :: "machine_word list \<Rightarrow> kernel_state \<Rightarrow> bool"
+where
+  "valid_global_pts' pts \<equiv> \<lambda>s. \<forall>p \<in> set pts. page_table_at' p s"
+
+definition
+  valid_global_pds' :: "machine_word list \<Rightarrow> kernel_state \<Rightarrow> bool"
+where
+  "valid_global_pds' pds \<equiv> \<lambda>s. \<forall>p \<in> set pds. page_directory_at' p s"
+
+definition
+  valid_global_pdpts' :: "machine_word list \<Rightarrow> kernel_state \<Rightarrow> bool"
+where
+  "valid_global_pdpts' pdpts \<equiv> \<lambda>s. \<forall>p \<in> set pdpts. pd_pointer_table_at' p s"
+
+definition
+  valid_x64_irq_state' :: "(8 word \<Rightarrow> x64irqstate) \<Rightarrow> bool"
+where
+  "valid_x64_irq_state' irqState \<equiv> \<forall>irq > maxIRQ. irqState irq = X64IRQFree"
+
+definition valid_ioapic_2 :: "machine_word \<Rightarrow> (machine_word \<Rightarrow> 8 word) \<Rightarrow> bool" where
+  "valid_ioapic_2 num_ioapics ioapic_nirqs \<equiv>
+    num_ioapics \<le> of_nat Kernel_Config.maxNumIOAPIC \<and>
+    (\<forall>ioapic < num_ioapics. 0 < ioapic_nirqs ioapic) \<and>
+    (\<forall>ioapic < num_ioapics. ioapic_nirqs ioapic \<le> ucast ioapicIRQLines) \<and>
+    (\<forall>ioapic > of_nat Kernel_Config.maxNumIOAPIC. ioapic_nirqs ioapic = 0)"
+
+abbreviation valid_ioapic where
+  "valid_ioapic s \<equiv>
+     valid_ioapic_2 (x64KSNumIOAPICs (ksArchState s)) (x64KSIOAPICnIRQs (ksArchState s))"
+
+lemmas valid_ioapic_def = valid_ioapic_2_def
 
 definition valid_arch_state' :: "kernel_state \<Rightarrow> bool" where
   "valid_arch_state' \<equiv> \<lambda>s.
-   valid_asid_table' (armKSASIDTable (ksArchState s)) \<and>
-   0 \<notin> ran (armKSVMIDTable (ksArchState s)) \<and>
-   (case armHSCurVCPU (ksArchState s) of
-      Some (v, b) \<Rightarrow> ko_wp_at' (is_vcpu' and hyp_live') v s
-      | _ \<Rightarrow> True) \<and>
-   armKSGICVCPUNumListRegs (ksArchState s) \<le> max_armKSGICVCPUNumListRegs \<and>
-   canonical_address (addrFromKPPtr (armKSGlobalUserVSpace (ksArchState s)))"
+  valid_asid_table' (x64KSASIDTable (ksArchState s)) s \<and>
+  valid_cr3' (x64KSCurrentUserCR3 (ksArchState s)) \<and>
+  page_map_l4_at' (x64KSSKIMPML4 (ksArchState s)) s \<and>
+  valid_global_pds' (x64KSSKIMPDs (ksArchState s)) s \<and>
+  valid_global_pdpts' (x64KSSKIMPDPTs (ksArchState s)) s \<and>
+  valid_global_pts' (x64KSSKIMPTs (ksArchState s)) s \<and>
+  valid_x64_irq_state' (x64KSIRQState (ksArchState s)) \<and>
+  valid_ioapic s"
+
+definition cap_ioports' :: "capability \<Rightarrow> ioport set" where
+  "cap_ioports' c \<equiv> case c of
+    ArchObjectCap (IOPortCap f l) \<Rightarrow> {f..l}
+  | _ \<Rightarrow> {}"
+
+definition issued_ioports' :: "Arch.kernel_state \<Rightarrow> ioport set" where
+  "issued_ioports' \<equiv> \<lambda>as. Collect (x64KSAllocatedIOPorts as)"
+
+definition all_ioports_issued' :: "(machine_word \<Rightarrow> capability option) \<Rightarrow> Arch.kernel_state \<Rightarrow> bool"
+   where
+  "all_ioports_issued' \<equiv> \<lambda>cs as. \<forall>cap \<in> ran cs. cap_ioports' cap \<subseteq> issued_ioports' as"
 
 definition archMakeObjectT :: "arch_kernel_object_type \<Rightarrow> kernel_object" where
   "archMakeObjectT atp \<equiv>
      case atp
-     of PTET \<Rightarrow> injectKO (makeObject :: pte)
-      | ASIDPoolT \<Rightarrow> injectKO (makeObject :: asidpool)
-      | VCPUT \<Rightarrow> injectKO (makeObject :: vcpu)"
+     of PDET \<Rightarrow> injectKO (makeObject :: pde)
+      | PTET \<Rightarrow> injectKO (makeObject :: pte)
+      | PDPTET \<Rightarrow> injectKO (makeObject :: pdpte)
+      | PML4ET \<Rightarrow> injectKO (makeObject :: pml4e)
+      | ASIDPoolT \<Rightarrow> injectKO (makeObject :: asidpool)"
 
 end
 end
