proof/refine/X64/Detype_R.thy
@@ -405,13 +405,13 @@ lemma cte_wp_at_delete':
   apply (drule(1) aligned_ranges_subset_or_disjoint)
   apply (subgoal_tac "{p, p - n} \<subseteq> obj_range' (p - n) (KOTCB obj)")
    apply (clarsimp simp del: atLeastAtMost_iff
-                       simp: field_simps objBits_simps obj_range'_def)
+                       simp: field_simps objBits_simps obj_range'_def mask_def)
    apply fastforce
-  apply (simp add: obj_range'_def mask_in_range[symmetric]
+  apply (simp add: obj_range'_def neg_mask_in_mask_range[symmetric]
               del: atLeastAtMost_iff)
   apply (simp add: objBits_simps)
   apply (frule(1) tcb_cte_cases_aligned_helpers)
-  apply (simp add: is_aligned_neg_mask_eq)
+  apply simp
   done
 
 lemma map_to_ctes_delete:
@@ -911,7 +911,7 @@ lemma detype_tcbSchedNexts_of:
   apply (clarsimp simp: opt_map_def)
   apply (rule ext)
   apply (rename_tac s)
-  apply (clarsimp simp: ko_wp_at'_def split: option.splits)
+  apply (clarsimp simp: ko_wp_at'_def live'_def split: option.splits)
   apply (drule_tac x=s in spec)
   apply force
   done
@@ -925,7 +925,7 @@ lemma detype_tcbSchedPrevs_of:
   apply (clarsimp simp: opt_map_def)
   apply (rule ext)
   apply (rename_tac s)
-  apply (clarsimp simp: ko_wp_at'_def split: option.splits)
+  apply (clarsimp simp: ko_wp_at'_def live'_def split: option.splits)
   apply (drule_tac x=s in spec)
   apply force
   done
@@ -939,7 +939,7 @@ lemma detype_inQ:
   apply (clarsimp simp: opt_map_def)
   apply (rule ext)
   apply (rename_tac s)
-  apply (clarsimp simp: inQ_def opt_pred_def ko_wp_at'_def split: option.splits)
+  apply (clarsimp simp: inQ_def opt_pred_def ko_wp_at'_def live'_def split: option.splits)
   apply (drule_tac x=s in spec)
   apply force
   done
@@ -1121,22 +1121,23 @@ lemma valid_obj':
       apply fastforce
      apply simp
     apply (intro conjI)
+        apply (rename_tac tcb)
+        apply (case_tac "tcbState tcb"; clarsimp simp: valid_tcb_state'_def  dest!: refs_notRange)
        apply (rename_tac tcb)
-       apply (case_tac "tcbState tcb"; clarsimp simp: valid_tcb_state'_def  dest!: refs_notRange)
-      apply (rename_tac tcb)
-      apply (case_tac "tcbState tcb";
-             clarsimp simp: valid_tcb_state'_def valid_bound_ntfn'_def
-                     dest!: refs_notRange split: option.splits)
+       apply (case_tac "tcbState tcb";
+              clarsimp simp: valid_tcb_state'_def valid_bound_ntfn'_def
+                      dest!: refs_notRange split: option.splits)
+      apply (clarsimp simp: none_top_bool_cases)
+      apply (rename_tac prev)
+      apply (cut_tac P=live' and p=prev in live_notRange; fastforce?)
+      apply (fastforce dest: sym_heapD2[where p'=p]
+                       simp: opt_map_def ko_wp_at'_def obj_at'_def live'_def projectKOs)
      apply (clarsimp simp: none_top_bool_cases)
-     apply (rename_tac prev)
-     apply (cut_tac P=live' and p=prev in live_notRange; fastforce?)
-     apply (fastforce dest: sym_heapD2[where p'=p]
-                      simp: opt_map_def ko_wp_at'_def obj_at'_def projectKOs)
-    apply (clarsimp simp: none_top_bool_cases)
-    apply (rename_tac "next")
-    apply (cut_tac P=live' and p="next" in live_notRange; fastforce?)
-    apply (fastforce dest!: sym_heapD1[where p=p]
-                     simp: opt_map_def ko_wp_at'_def obj_at'_def projectKOs)
+     apply (rename_tac "next")
+     apply (cut_tac P=live' and p="next" in live_notRange; fastforce?)
+     apply (fastforce dest!: sym_heapD1[where p=p]
+                      simp: opt_map_def ko_wp_at'_def obj_at'_def live'_def projectKOs)
+    apply (clarsimp simp: valid_arch_tcb'_def)
    apply (clarsimp simp: valid_cte'_def)
    apply (rule_tac p=p in valid_cap2)
    apply (clarsimp simp: ko_wp_at'_def objBits_simps' cte_level_bits_def[symmetric])
@@ -1168,7 +1169,7 @@ lemma tcbSchedNexts_of_pspace':
    apply (case_tac "ksPSpace s' p"; clarsimp)
    apply (rename_tac obj)
    apply (case_tac "tcb_of' obj"; clarsimp)
-   apply (clarsimp simp: ko_wp_at'_def obj_at'_def)
+   apply (clarsimp simp: ko_wp_at'_def obj_at'_def live'_def)
    apply (fastforce simp: pspace_alignedD' pspace_distinctD')
   apply (clarsimp simp: opt_map_def split: option.splits)
   done
@@ -1185,14 +1186,15 @@ lemma tcbSchedPrevs_of_pspace':
    apply (case_tac "ksPSpace s' p"; clarsimp)
    apply (rename_tac obj)
    apply (case_tac "tcb_of' obj"; clarsimp)
-   apply (clarsimp simp: ko_wp_at'_def obj_at'_def)
+   apply (clarsimp simp: ko_wp_at'_def obj_at'_def live'_def)
    apply (fastforce simp: pspace_alignedD' pspace_distinctD')
   apply (clarsimp simp: opt_map_def split: option.splits)
   done
 
 lemma st_tcb:
   "\<And>P p. \<lbrakk> st_tcb_at' P p s'; \<not> P Inactive; \<not> P IdleThreadState \<rbrakk> \<Longrightarrow> st_tcb_at' P p state'"
-  by (fastforce simp: pred_tcb_at'_def obj_at'_real_def projectKOs dest: live_notRange)
+  by (fastforce simp: pred_tcb_at'_def obj_at'_real_def projectKOs live'_def hyp_live'_def
+                dest: live_notRange)
 
 lemma irq_nodes_global:
     "\<forall>irq :: 8 word. irq_node' s + (ucast irq) * 32 \<in> global_refs' s" (*2^cte_level_bits *)
@@ -1233,7 +1235,7 @@ proof -
     apply (frule valid_capAligned)
     apply (case_tac "\<exists>irq. cteCap c = IRQHandlerCap irq")
      apply (insert irq_nodes_range)[1]
-     apply clarsimp
+     apply (clarsimp simp: cteSizeBits_def shiftl_t2n')
     apply (frule subsetD [OF cte_refs_capRange])
       apply simp
      apply assumption
@@ -1569,7 +1571,9 @@ proof (simp add: invs'_def valid_state'_def valid_pspace'_def
 
   show "valid_irq_node' (irq_node' s') ?s"
     using virq irq_nodes_range
-    by (simp add: valid_irq_node'_def mult.commute mult.left_commute ucast_ucast_mask_8)
+    (* FIXME arch-split: where is the mismatch between cteSizeBits/shifts and actual numbers? *)
+    by (simp add: valid_irq_node'_def mult.commute mult.left_commute ucast_ucast_mask_8
+                  cteSizeBits_def shiftl_t2n')
 
   show "valid_irq_handlers' ?s" using virqh
     apply (simp add: valid_irq_handlers'_def irq_issued'_def
@@ -1583,7 +1587,7 @@ proof (simp add: invs'_def valid_state'_def valid_pspace'_def
     by (clarsimp simp: irq_control_def)
 
   from ioport_ctrl
-  show "ioport_control ?ctes'"
+  show "valid_arch_mdb_ctes ?ctes'"
     by (clarsimp simp: ioport_control_def)
 
   from dist_z
@@ -1657,7 +1661,7 @@ proof (simp add: invs'_def valid_state'_def valid_pspace'_def
     apply (frule if_live_then_nonz_capE'[OF iflive, OF ko_wp_at'_weakenE])
      apply (clarsimp simp: projectKOs)
      apply (case_tac "tcbState obj")
-            apply (clarsimp simp: projectKOs)+
+            apply (clarsimp simp: projectKOs live'_def)+
     apply (clarsimp dest!: ex_nonz_cap_notRange)
     done
 
@@ -1675,7 +1679,7 @@ proof (simp add: invs'_def valid_state'_def valid_pspace'_def
     apply (frule if_live_then_nonz_capE'[OF iflive, OF ko_wp_at'_weakenE])
      apply (clarsimp simp: projectKOs)
      apply (case_tac "tcbState obj")
-            apply (clarsimp simp: projectKOs)+
+            apply (clarsimp simp: projectKOs live'_def)+
     apply (clarsimp dest!: ex_nonz_cap_notRange elim!: ko_wp_at'_weakenE)
     done
 
@@ -1834,7 +1838,7 @@ lemma deleteObjects_st_tcb_at':
     apply (rule conjI)
      apply (fastforce elim: ko_wp_at'_weakenE)
     apply (erule if_live_then_nonz_capD' [rotated])
-     apply (clarsimp simp: projectKOs)
+     apply (clarsimp simp: projectKOs live'_def)
     apply (clarsimp simp: invs'_def valid_state'_def)
    apply (clarsimp simp: pred_tcb_at'_def obj_at'_real_def
                   field_simps ko_wp_at'_def ps_clear_def
@@ -1869,11 +1873,12 @@ lemma deleteObjects_cap_to':
   apply (simp add: delete_locale_def)
   done
 
+(* FIXME arch-split: consider "- mask_range ptr bits" in conclusion *)
 lemma valid_untyped_no_overlap:
   "\<lbrakk> valid_untyped' d ptr bits idx s; is_aligned ptr bits; valid_pspace' s \<rbrakk>
   \<Longrightarrow> pspace_no_overlap' ptr bits (s\<lparr>ksPSpace := ksPSpace s |` (- {ptr .. ptr + 2 ^ bits - 1})\<rparr>)"
   apply (clarsimp simp del: atLeastAtMost_iff
-            simp: pspace_no_overlap'_def valid_cap'_def valid_untyped'_def is_aligned_neg_mask_eq)
+            simp: pspace_no_overlap'_def valid_cap'_def valid_untyped'_def)
   apply (drule_tac x=x in spec)
   apply (drule restrict_map_Some_iff[THEN iffD1])
   apply clarsimp
@@ -1885,10 +1890,10 @@ lemma valid_untyped_no_overlap:
   apply (drule (1) aligned_ranges_subset_or_disjoint)
   apply (clarsimp simp del: Int_atLeastAtMost atLeastAtMost_iff atLeastatMost_subset_iff)
   apply (elim disjE)
-    apply (subgoal_tac "ptr \<in> {x..x + 2 ^ objBitsKO ko - 1}")
-     apply (clarsimp simp:p_assoc_help)
-    apply (clarsimp simp:p_assoc_help)
-   apply fastforce+
+    apply (subgoal_tac "ptr \<in> mask_range x (objBitsKO ko)")
+     apply (clarsimp simp:p_assoc_help mask_def)
+    apply (clarsimp simp:p_assoc_help mask_def)
+   apply (fastforce simp: mask_def add_diff_eq)+
   done
 
 lemma deleteObject_no_overlap[wp]:
@@ -2619,11 +2624,11 @@ lemma placeNewObject_modify_commute:
     apply (case_tac "x = ptr'")
      apply (subgoal_tac "objBitsKO koa = objBitsKO ko")
       apply (drule(1) pspace_no_overlapD')
-      apply (clarsimp simp:field_simps)
+      apply (clarsimp simp:field_simps mask_def)
      apply (clarsimp)
     apply (drule_tac x = x and s = s in pspace_no_overlapD'[rotated])
      apply (simp)
-    apply (clarsimp simp:field_simps)
+    apply (clarsimp simp:field_simps mask_def)
   apply (subgoal_tac "pspace_aligned'
     (ksPSpace_update (\<lambda>ps. ps(ptr' \<mapsto> f (ps ptr'))) s)")
   prefer 2
@@ -2769,10 +2774,10 @@ lemma getPDE_det:
    apply (rule conjI)
     apply (subst add.commute)
     apply (rule word_diff_ls')
-     apply (clarsimp simp: not_le plus_one_helper)
+     apply (clarsimp simp: not_le plus_one_helper mask_def)
     apply (subst add.commute)
-    apply (simp add: is_aligned_no_wrap' is_aligned_mask)
-  apply auto
+    apply (subst is_aligned_no_wrap'[simplified is_aligned_mask], assumption; simp add: mask_def)
+   apply auto
   done
 
 lemma in_dom_eq:
@@ -2915,9 +2920,9 @@ lemma modify_pde_psp_no_overlap':
   apply (intro allI impI)
   apply (clarsimp split:if_splits)
    apply (drule(1) pspace_no_overlapD')
-    apply (simp add:objBits_simps archObjSize_def field_simps)
+    apply (simp add:objBits_simps archObjSize_def field_simps mask_def)
   apply (drule(1) pspace_no_overlapD')+
-  apply (simp add:field_simps)
+  apply (simp add:field_simps mask_def)
   done
   qed
 
@@ -3054,11 +3059,10 @@ lemma getPML4E_det:
    apply (rule conjI)
     apply (subst add.commute)
     apply (rule word_diff_ls')
-     apply (clarsimp simp:field_simps not_le plus_one_helper)
+     apply (clarsimp simp:field_simps not_le plus_one_helper mask_def)
     apply (subst add.commute)
-    apply (simp add: is_aligned_no_wrap' is_aligned_mask)
-   apply simp
-  apply auto
+    apply (subst is_aligned_no_wrap'[simplified is_aligned_mask], assumption; simp add: mask_def)
+   apply auto
   done
 
 lemma setCTE_pml4e_at':
@@ -3257,9 +3261,9 @@ lemma modify_pml4e_psp_no_overlap':
   apply (intro allI impI)
   apply (clarsimp split:if_splits)
    apply (drule(1) pspace_no_overlapD')
-    apply (simp add:objBits_simps archObjSize_def field_simps)
+    apply (simp add:objBits_simps archObjSize_def field_simps mask_def)
   apply (drule(1) pspace_no_overlapD')+
-  apply (simp add:field_simps)
+  apply (simp add:field_simps mask_def)
   done
   qed
 
@@ -3570,8 +3574,8 @@ lemma getTCB_det:
    apply (rule conjI)
     apply (subst add.commute)
     apply (rule word_diff_ls')
-     apply (clarsimp simp:field_simps not_le plus_one_helper)
-    apply (simp add:field_simps is_aligned_no_wrap' is_aligned_mask)
+     apply (clarsimp simp:field_simps not_le plus_one_helper mask_def)
+    apply (simp add:field_simps is_aligned_no_overflow_mask flip: is_aligned_mask)
    apply simp
   apply auto
   done
@@ -3704,7 +3708,7 @@ lemma placeNewObject_tcb_at':
   apply (wp unless_wp |wpc | simp add:alignError_def)+
   by (auto simp: obj_at'_def is_aligned_mask lookupAround2_None1
                     lookupAround2_char1 field_simps objBits_simps
-                    projectKO_opt_tcb projectKO_def return_def ps_clear_def
+                    projectKO_opt_tcb projectKO_def return_def ps_clear_def add_mask_fold
            split: if_splits
            dest!: pspace_no_overlap_disjoint')
 
@@ -3828,8 +3832,7 @@ lemma ctes_of_ko_at:
   (\<exists>ptr ko. (ksPSpace s ptr = Some ko \<and> p \<in> obj_range' ptr ko))"
   apply (clarsimp simp: map_to_ctes_def Let_def split: if_split_asm)
    apply (intro exI conjI, assumption)
-   apply (simp add: obj_range'_def objBits_simps' add.commute)
-   apply (simp add: is_aligned_no_wrap')
+   apply (simp add: obj_range'_def objBits_simps' is_aligned_no_overflow_mask)
   apply (intro exI conjI, assumption)
   apply (clarsimp simp: objBits_simps' obj_range'_def word_and_le2)
   apply (thin_tac "P" for P)+
@@ -3845,7 +3848,7 @@ lemma pspace_no_overlapD2':
    apply clarsimp
    apply (drule(1) pspace_no_overlapD')
    apply (erule in_empty_interE)
-    apply (simp add:obj_range'_def)
+    apply (simp add:obj_range'_def add_mask_fold)
     apply clarsimp
     apply (subst is_aligned_neg_mask_eq[symmetric])
     apply simp
@@ -4204,7 +4207,7 @@ proof -
       apply (rule is_aligned_shiftl_self)
      apply (simp add:range_cover_def)
     apply simp
-    apply (simp add:word_le_sub1 shiftl_t2n field_simps)
+    apply (simp add:word_le_sub1 shiftl_t2n field_simps mask_def)
     done
 qed
 
@@ -4283,29 +4286,27 @@ lemma pspace_no_overlap'_le:
   assumes b: "sz < word_bits"
   shows "pspace_no_overlap' ptr sz' s"
   proof -
-  note blah[simp del] = untyped_range.simps usable_untyped_range.simps atLeastAtMost_iff atLeastatMost_subset_iff atLeastLessThan_iff
-          Int_atLeastAtMost atLeastatMost_empty_iff split_paired_Ex
+  note no_simps [simp del] = untyped_range.simps usable_untyped_range.simps atLeastAtMost_iff
+                             atLeastatMost_subset_iff atLeastLessThan_iff
+                             Int_atLeastAtMost atLeastatMost_empty_iff split_paired_Ex
   have diff_cancel: "\<And>a b c. (a::machine_word) + b - c = b + (a - c)"
    by simp
-  have bound :"(ptr && ~~ mask sz') - (ptr && ~~ mask sz) \<le> 2 ^ sz - 2 ^ sz'"
-    by (rule neg_mask_diff_bound[OF psp(2)])
+  have bound: "(ptr && ~~ mask sz') - (ptr && ~~ mask sz) \<le> mask sz - mask sz'"
+    using neg_mask_diff_bound[OF psp(2)]
+    by (simp add: mask_def)
   show ?thesis
-  using psp
+    using psp
     apply (clarsimp simp:pspace_no_overlap'_def)
     apply (drule_tac x = x in spec)
     apply clarsimp
     apply (erule disjoint_subset2[rotated])
-    apply (clarsimp simp:blah)
-    apply (rule word_plus_mcs[OF _  is_aligned_no_overflow'])
+    apply (clarsimp simp: no_simps)
+    apply (rule word_plus_mcs[OF _  is_aligned_no_overflow_mask])
      apply (simp add:diff_cancel p_assoc_help)
      apply (rule le_plus)
-      apply (simp add:field_simps)
       apply (rule bound)
-     apply (rule word_le_minus_mono_left)
-      apply (erule two_power_increasing[OF _ b[unfolded word_bits_def]])
-     apply (rule word_1_le_power)
-     using b[unfolded word_bits_def] apply simp
-    apply (simp add:is_aligned_neg_mask)
+     apply (erule mask_mono)
+    apply simp
     done
 qed
 
@@ -5028,7 +5029,7 @@ proof -
     apply (drule(1) pspace_no_overlapD')
    apply (subst (asm) range_cover_tail_mask)
     apply simp+
-   apply (simp add:word_le_sub1 shiftl_t2n field_simps)
+   apply (simp add:word_le_sub1 shiftl_t2n field_simps mask_def)
   apply auto
   done
 qed
